progress on upsert

templates/multicopy/general_multicopy.v
@@ -7,7 +7,7 @@ From iris.proofmode Require Import tactics.
 From iris.heap_lang Require Import proofmode par.
 From iris.bi.lib Require Import fractional.
 Set Default Proof Using "All".
-Require Export KT_flows inset_flows_multicopy.
+Require Export KT_flows inset_flows_multicopy auth_ext.
 
 (** Algorithms **)
 
@@ -38,7 +38,7 @@ Definition traverse : val :=
   rec: "t_rec" "n" "k" :=
     lockNode "n" ;;
     let: "t" := inContents "n" "k" in
-    if: "t" ≠ #0 
+    if: ("t" ≠ #0%nat)%nat 
     then
       unlockNode "n";; "t"
     else
@@ -121,11 +121,56 @@ Section multicopy.
   Instance node_timeless r n es C: Timeless (node r n es C).
   Proof. apply node_timeless_proof. Qed.
 
+  Hypothesis node_sep_star: ∀ r n es C es' C',
+    node r n es C ∗ node r n es' C' -∗ False.
+
+
+  Definition out_edgeset_list (k: K) (esl : list (Node * gset K)) :=             
+    list_find (λ ns, k ∈ ns.2) esl.
+
+  Definition out_edgeset (k: K) (es: esT) : bool := 
+    match (out_edgeset_list k (map_to_list es)) with
+    | None => false
+    | _ => true end.
+
+  Lemma out_edgeset_true k : ∀ es, out_edgeset k es = true → ∃ n, k ∈ es !!! n.
+  Proof.
+    intros es Hes.
+    unfold out_edgeset in Hes.
+    destruct (out_edgeset_list k (map_to_list es)) 
+      as [ (i, (n,s)) | ] eqn: E; try inversion Hes.
+    unfold out_edgeset_list in E.
+    rewrite list_find_Some in E *; intros E.
+    destruct E as [E1 [E2 _]].
+    simpl in E2. apply elem_of_list_lookup_2 in E1.
+    apply elem_of_map_to_list in E1.
+    exists n. rewrite /(es !!! n). 
+    unfold finmap_lookup_total. rewrite E1. by simpl.
+  Qed.
+      
+  Lemma out_edgeset_false k : ∀ es, out_edgeset k es = false → ∀ n, k ∉ es !!! n.
+  Proof.
+    intros es Hes n.
+    unfold out_edgeset in Hes.
+    destruct (out_edgeset_list k (map_to_list es)) 
+      as [ p | ] eqn: E; try inversion Hes.
+    unfold out_edgeset_list in E.
+    rewrite list_find_None in E *; intros E.
+    rewrite Forall_forall in E *; intros E.
+    rewrite /(es !!! n). 
+    unfold finmap_lookup_total.
+    destruct (es !! n) eqn:F.
+    - rewrite F. simpl.
+      rewrite <-(elem_of_map_to_list es n g) in F.
+      pose proof E (n, g) F as E. by simpl in E.
+    - rewrite F. simpl. set_solver.
+  Qed.    
+
   Definition inFP γ_f (n: Node) : iProp := own γ_f (◯ {[n]}).
 
   Definition closed γ_f (es: esT) : iProp := ∀ n, ⌜es !!! n  ≠ ∅⌝ → inFP γ_f n.
 
-  Definition inflow_zero (I: KT_flowint_ur K) : iProp := ⌜∀ n, inf I n = ∅⌝. 
+  Definition inflow_zero (I: KT_flowint_ur K) : iProp := ⌜∀ n, inset_KT I n = ∅⌝. 
 
   Definition inflow_R (R: inset_flowint_ur K) r : iProp := 
     ⌜∀ n k, if n =? r then in_inset K k R n else ¬ in_inset K k R n⌝. 
@@ -133,12 +178,12 @@ Section multicopy.
   Definition outflow_constraint_I (In: KT_flowint_ur K) (es: esT) 
                           (Cn Bn: gmap K natUR) : iProp := 
     ⌜∀ n' k t, (k,t) ∈ outset_KT In n' ↔ 
-                          k ∈ es !!! n' ∧ (Cn !!! k = 0) ∧ (Bn !! k = Some(t))⌝.
+                          k ∈ es !!! n' ∧ (Cn !!! k = 0) ∧ (Bn !!! k = t)⌝.
 
   Definition outflow_constraint_J (Jn: KT_flowint_ur K) (es: esT) 
                           (Cn Bn: gmap K natUR) : iProp := 
     ⌜∀ n' k t, (k,t) ∈ outset_KT Jn n' ↔ 
-                          k ∈ es !!! n' ∧ (Cn !! k = Some(t))⌝.
+                          k ∈ es !!! n' ∧ (Cn !!! k = t)⌝.
 
   Definition outflow_constraint_R (Rn: inset_flowint_ur K) (es: esT) n : iProp := 
     ⌜∀ n' k, in_outset K k Rn n' ↔ k ∈ es !!! n' ∧ in_inset K k Rn n⌝.
@@ -156,7 +201,7 @@ Section multicopy.
               ⌜∀ k t, (k,t) ∈ inset_KT In n → Bn !!! k = t⌝.
 
   Definition φ3 n (Bn: gmap K natUR) Jn : iProp :=
-              ⌜∀ k t, (k,t) ∈ inset_KT Jn n → t ≤ Bn !!! k⌝.
+              ⌜∀ k t, (k,t) ∈ inset_KT Jn n → Bn !!! k ≤ t⌝.
 
   Definition φ4 n (Bn: gmap K natUR) Rn : iProp :=
               ⌜∀ k, Bn !! k = None ∨ in_inset K k Rn n⌝.
@@ -207,7 +252,8 @@ Section multicopy.
     ∗ inFP γ_f n
     ∗ closed γ_f es
     ∗ outflow_constraints n In Jn Rn es Cn Bn
-    ∗ (if (n =? r) then ⌜Bn = map_of_set H⌝ ∗ inflow_zero In else True)%I
+    ∗ (if (n =? r) then ⌜Bn = map_of_set H⌝ ∗ inflow_zero In ∗ inflow_zero Jn 
+                   else True)%I
     ∗ ([∗ set] k ∈ KS, own (γ_cir n k) (● (MaxNat (Bn !!! k))))
     ∗ φ1 Bn Cn In ∗ φ2 n Bn In 
     ∗ φ3 n Bn Jn ∗ φ4 n Bn Rn ∗ φ5 n Rn. 
@@ -307,12 +353,231 @@ Section multicopy.
                   node r r es Cn' ∗ if succ then ⌜Cn' = <[k := t]> Cn⌝ 
                                 else ⌜Cn' = Cn⌝ }}})%I.
 
-
-  (** Proofs **)  
+  (** Useful lemmas and definitions **)
 
   Instance test r n γ_t T : Laterable (if n =? r then 
                                             own γ_t (●{1 / 2} T) else ⌜True⌝)%I.
   Proof. Admitted.
+
+  Lemma inFP_domm γ_f n D : inFP γ_f n -∗ own γ_f (● D) -∗ ⌜n ∈ D⌝.
+  Proof.
+    iIntros "FP HD".
+    iPoseProof (own_valid_2 _ _ _ with "[$HD] [$FP]") as "H'".
+    iDestruct "H'" as %H'.
+    apply auth_both_valid_discrete in H'.
+    destruct H' as [H' _].
+    apply gset_included in H'.
+    iPureIntro. set_solver.
+  Qed.
+  
+  Lemma frac_eq γ_e γ_c γ_b n es Cn Bn es' Cn' Bn' : 
+              frac_ghost_state γ_e γ_c γ_b n es Cn Bn -∗
+                  frac_ghost_state γ_e γ_c γ_b n es' Cn' Bn'-∗ 
+                    ⌜es = es'⌝ ∗ ⌜Cn = Cn'⌝ ∗ ⌜Bn = Bn'⌝.
+  Proof.
+    iIntros "H1 H2". unfold frac_ghost_state.
+    iDestruct "H1" as "(H1_es & H1_c & H1_b)".
+    iDestruct "H2" as "(H2_es & H2_c & H2_b)".
+    iPoseProof (own_valid_2 _ _ _ with "[$H1_es] [$H2_es]") as "Hes".
+    iPoseProof (own_valid_2 _ _ _ with "[$H1_c] [$H2_c]") as "Hc".
+    iPoseProof (own_valid_2 _ _ _ with "[$H1_b] [$H2_b]") as "Hb".
+    iDestruct "Hes" as %Hes. iDestruct "Hc" as %Hc. iDestruct "Hb" as %Hb.
+    apply frac_agree_op_valid in Hes. destruct Hes as [_ Hes].
+    apply frac_agree_op_valid in Hc. destruct Hc as [_ Hc].
+    apply frac_agree_op_valid in Hb. destruct Hb as [_ Hb].
+    apply leibniz_equiv_iff in Hes.
+    apply leibniz_equiv_iff in Hc. 
+    apply leibniz_equiv_iff in Hb.
+    iPureIntro. repeat split; try done.   
+  Qed.
+
+  Lemma frac_update γ_e γ_c γ_b r es Cr Br es' Cr' Br' : 
+              frac_ghost_state γ_e γ_c γ_b r es Cr Br ∗ 
+                 frac_ghost_state γ_e γ_c γ_b r es Cr Br ==∗ 
+                      frac_ghost_state γ_e γ_c γ_b r es' Cr' Br' ∗ 
+                        frac_ghost_state γ_e γ_c γ_b r es' Cr' Br'.
+  Proof.
+    iIntros "(H1 & H2)". 
+    iDestruct "H1" as "(H1_es & H1_c & H1_b)".
+    iDestruct "H2" as "(H2_es & H2_c & H2_b)".
+    iCombine "H1_es H2_es" as "Hes". 
+    iEval (rewrite <-frac_agree_op) in "Hes". 
+    iEval (rewrite Qp_half_half) in "Hes". 
+    iCombine "H1_c H2_c" as "Hc". 
+    iEval (rewrite <-frac_agree_op) in "Hc". 
+    iEval (rewrite Qp_half_half) in "Hc". 
+    iCombine "H1_b H2_b" as "Hb". 
+    iEval (rewrite <-frac_agree_op) in "Hb". 
+    iEval (rewrite Qp_half_half) in "Hb".
+    iMod ((own_update (γ_e r) (to_frac_agree 1 es) 
+                  (to_frac_agree 1 es')) with "[$Hes]") as "Hes".
+    { apply cmra_update_exclusive. 
+      unfold valid, cmra_valid. simpl. unfold prod_valid.
+      split; simpl; try done. }
+    iEval (rewrite <-Qp_half_half) in "Hes".
+    iEval (rewrite frac_agree_op) in "Hes".  
+    iDestruct "Hes" as "(H1_es & H2_es)".            
+    iMod ((own_update (γ_c r) (to_frac_agree 1 Cr) 
+                  (to_frac_agree 1 Cr')) with "[$Hc]") as "Hc".
+    { apply cmra_update_exclusive. 
+      unfold valid, cmra_valid. simpl. unfold prod_valid.
+      split; simpl; try done. }
+    iEval (rewrite <-Qp_half_half) in "Hc".
+    iEval (rewrite frac_agree_op) in "Hc".  
+    iDestruct "Hc" as "(H1_c & H2_c)".
+    iMod ((own_update (γ_b r) (to_frac_agree 1 Br) 
+                  (to_frac_agree 1 Br')) with "[$Hb]") as "Hb".
+    { apply cmra_update_exclusive. 
+      unfold valid, cmra_valid. simpl. unfold prod_valid.
+      split; simpl; try done. }
+    iEval (rewrite <-Qp_half_half) in "Hb".
+    iEval (rewrite frac_agree_op) in "Hb".  
+    iDestruct "Hb" as "(H1_b & H2_b)".
+  iModIntro. iFrame.
+  Qed.
+
+  Definition outflow_insert_KT (I : KT_flowint_ur K) (n: Node) 
+                              (k: K) (t: nat) :KT_flowint_ur K := 
+             let I_out_n := ((nzmap_imerge 
+                         (λ k' a1 _, if (decide (k' = (k, t))) then 1 else a1)
+                         (out I n) (∅)): (KT_multiset)) in
+             let I'_out := ((nzmap_imerge 
+                          (λ k' a1 _, if (decide (k = n)) then I_out_n else a1)
+                          (out_map I) (∅)) : (nzmap Node KT_multiset)) in
+             (int {| infR := inf_map I ; outR := I'_out |}).              
+
+  Definition outflow_delete_KT (I : KT_flowint_ur K) (n: Node) 
+                              (k: K) (t: nat) :KT_flowint_ur K := 
+             let I_out_n := ((nzmap_imerge 
+                         (λ k' a1 _, if (decide (k' = (k, t))) then 0 else a1)
+                         (out I n) (∅)): (KT_multiset)) in
+             let I'_out := ((nzmap_imerge 
+                          (λ k' a1 _, if (decide (k = n)) then I_out_n else a1)
+                          (out_map I) (∅)) : (nzmap Node KT_multiset)) in
+             (int {| infR := inf_map I ; outR := I'_out |}).
+
+  Lemma outflow_insert_outset_KT I n k t I' :
+        I' = outflow_insert_KT I n k t → 
+           ∀ n', (n' = n → outset_KT I' n' = (outset_KT I n') ∪ {[(k,t)]})
+               ∧ (n' ≠ n → outset_KT I' n' = outset_KT I n').
+  Proof.
+  Admitted.
+
+  Lemma outflow_delete_outset_KT I n k t I' :
+        I' = outflow_delete_KT I n k t → 
+           ∀ n', (n' = n → outset_KT I' n' = (outset_KT I n') ∖ {[(k,t)]})
+               ∧ (n' ≠ n → outset_KT I' n' = outset_KT I n').
+  Proof.
+  Admitted.
+
+  Definition inflow_insert_KT (I : KT_flowint_ur K) (n: Node) 
+                              (k: K) (t: nat) :KT_flowint_ur K := 
+             let I_inf_n := ((nzmap_imerge 
+                         (λ k' a1 _, if (decide (k' = (k, t))) then 1 else a1)
+                         (inf I n) (∅)): (KT_multiset)) in
+             let I'_inf := (<[ n := I_inf_n ]>(inf_map I):(gmap Node KT_multiset)) in
+             (int {| infR := I'_inf ; outR := out_map I |}).              
+
+  Definition inflow_delete_KT (I : KT_flowint_ur K) (n: Node) 
+                              (k: K) (t: nat) :KT_flowint_ur K := 
+             let I_inf_n := ((nzmap_imerge 
+                         (λ k' a1 _, if (decide (k' = (k, t))) then 0 else a1)
+                         (inf I n) (∅)): (KT_multiset)) in
+             let I'_inf := (<[ n := I_inf_n ]>(inf_map I):(gmap Node KT_multiset)) in
+             (int {| infR := I'_inf ; outR := out_map I |}).           
+
+  Lemma inflow_insert_outset_KT I n k t I' :
+        I' = inflow_insert_KT I n k t → 
+           ∀ n', (n' = n → inset_KT I' n' = (inset_KT I n') ∪ {[(k,t)]})
+               ∧ (n' ≠ n → inset_KT I' n' = inset_KT I n').
+  Proof.
+  Admitted.
+
+  Lemma inflow_delete_outset_KT I n k t I' :
+        I' = inflow_delete_KT I n k t → 
+           ∀ n', (n' = n → inset_KT I' n' = (inset_KT I n') ∖ {[(k,t)]})
+               ∧ (n' ≠ n → inset_KT I' n' = inset_KT I n').
+  Proof.
+  Admitted.
+
+
+  Lemma inflow_insert_domm I n k t I' : 
+        I' = inflow_insert_KT I n k t → domm I' = domm I.
+  Proof.
+  Admitted.
+
+  Lemma inflow_delete_domm I n k t I' : 
+        I' = inflow_delete_KT I n k t → domm I' = domm I.
+  Proof.
+  Admitted.
+
+  Lemma flow_delete_eq_KT I1 I1' I2 I2' n k t :
+        I1' = outflow_delete_KT I1 n k t →
+          I2' = inflow_delete_KT I2 n k t →
+            I1 ⋅ I2 = I1' ⋅ I2'.
+  Proof.
+  Admitted.    
+
+  Lemma flow_insert_eq_KT I1 I1' I2 I2' n k t :
+        I1' = outflow_insert_KT I1 n k t →
+          I2' = inflow_insert_KT I2 n k t →
+            I1 ⋅ I2 = I1' ⋅ I2'.
+  Proof.
+  Admitted.    
+
+  Lemma outflow_insert_inf_eq_KT I n k t I' :
+        I' = outflow_insert_KT I n k t → 
+          ∀ n', inset_KT I' n' = inset_KT I n'.
+  Proof.
+  Admitted.
+
+  Lemma outflow_delete_inf_eq_KT I n k t I' :
+        I' = outflow_delete_KT I n k t → 
+          ∀ n', inset_KT I' n' = inset_KT I n'.
+  Proof.
+  Admitted.
+  
+  Lemma auth_agree γ xs ys :
+    own γ (● (Excl' xs)) -∗ own γ (◯ (Excl' ys)) -∗ ⌜xs = ys⌝.
+  Proof.
+    iIntros "Hγ● Hγ◯". by iDestruct (own_valid_2 with "Hγ● Hγ◯")
+      as %[<-%Excl_included%leibniz_equiv _]%auth_both_valid_discrete.
+  Qed.
+
+  Lemma auth_agree' (γ: gname) (xs ys: gset KT) :
+    own γ (● (Excl' xs)) -∗ own γ (◯ (Excl' ys)) -∗ ⌜xs = ys⌝.
+  Proof.
+    iIntros "Hγ● Hγ◯". by iDestruct (own_valid_2 with "Hγ● Hγ◯")
+      as %[<-%Excl_included%leibniz_equiv _]%auth_both_valid_discrete.
+  Qed.
+
+
+  Lemma auth_update γ ys xs1 xs2 :
+    own γ (● (Excl' xs1)) -∗ own γ (◯ (Excl' xs2)) ==∗
+      own γ (● (Excl' ys)) ∗ own γ (◯ (Excl' ys)).
+  Proof.
+    iIntros "Hγ● Hγ◯".
+    iMod (own_update_2 _ _ _ (● Excl' ys ⋅ ◯ Excl' ys)
+      with "Hγ● Hγ◯") as "[$$]".
+    { by apply auth_update, option_local_update, exclusive_local_update. }
+    done.
+  Qed.
+  
+  Lemma auth_update' (γ: gname) (ys xs1 xs2: gset KT) :
+    own γ (● (Excl' xs1)) -∗ own γ (◯ (Excl' xs2)) ==∗
+      own γ (● (Excl' ys)) ∗ own γ (◯ (Excl' ys)).
+  Proof.
+    iIntros "Hγ● Hγ◯".
+    iMod (own_update_2 _ _ _ (● Excl' ys ⋅ ◯ Excl' ys)
+      with "Hγ● Hγ◯") as "[$$]".
+    { admit. }  
+    (* { apply auth_update. option_local_update, exclusive_local_update. } *)
+    done.
+  Admitted.
+
+
+  (** Proofs **)  
+
 
 (*
   Lemma traverse_spec γ_te γ_he γ_s γ_t γ_I γ_J γ_R 
@@ -325,40 +590,43 @@ Section multicopy.
                                              ∗ ⌜t0 ≤ t'⌝ , RET #t' >>>.
   Proof.
     iIntros "k_in_KS #HInv". iLöb as "IH" forall (n t1).
-    iIntros "#HFP_n #Hlb H". iDestruct "H" as %t0_le_t1.
+    iIntros "#FP_n #Hlb H". iDestruct "H" as %t0_le_t1.
     iDestruct "k_in_KS" as %k_in_KS.
     iIntros (Φ) "AU". wp_lam. wp_pures.
     awp_apply lockNode_spec_high; try done.
     iAaccIntro with ""; try eauto with iFrame. 
     iIntros (Cn Bn)"HnP_n". iModIntro.
-    wp_pures. iDestruct "HnP_n" as (es T)"(node_n & HnP_n')".
+    wp_pures. iDestruct "HnP_n" as (es T)"(node_n & HnP_frac & HnP_C & HnP_t)".
     wp_apply (inContents_spec with "node_n").
     iIntros (t) "(node_n & H)". iDestruct "H" as %Cn_val.
-    wp_pures. case_eq (bool_decide (#t = #0)).
+    wp_pures. case_eq (bool_decide ((#t = #0%nat)%nat)).
     - intros Ht. wp_pures.
       wp_apply (findNext_spec with "node_n").
       iIntros (b n1) "(node_n & Hif)". destruct b.
       + wp_pures. iDestruct "Hif" as %k_in_es.
         iApply fupd_wp. iInv "HInv" as ">H".
         iDestruct "H" as (T' H I J R) "(Hglob & Hstar)".
-        iAssert (⌜n ∈ domm I⌝)%I as "%". { admit. }
+        iAssert (⌜n ∈ domm I⌝)%I as "%". 
+        { iDestruct "Hglob" as "(MCS_auth & HH & Ht & HI & HJ & HR & Hf 
+                & Inf_I & Inf_J & Inf_R & _ & Max_ts & domm_IJ & domm_IR)".
+          by iPoseProof (inFP_domm _ _ _ with "[$FP_n] [$Hf]") as "H'". }
         (* { by iPoseProof (inFP_domm with "[$Hfp] [$Hdomm]") as "?". } *) 
         rewrite (big_sepS_delete _ (domm I) n); last by eauto.
         iDestruct "Hstar" as "(H_n & Hstar')".
         iDestruct "H_n" as (bn Cn' Bn')"(Hl_n & Hlif_n & HnS_n)".
-        iAssert (⌜Cn' = Cn⌝)%I as "%".  
-        { admit. } subst Cn'.
-        iAssert (⌜Bn' = Bn⌝)%I as "%".  
-        { admit. } subst Bn'.
-        iDestruct "HnS_n" as (es' In Jn Rn) 
-           "(HnS_frac & HnS_si & HnS_FP & HnS_cl & HnS_oc & HnS_H & HnS_star & Hφ)".
-        iAssert (⌜es' = es⌝)%I as "%".  
-        { admit. } subst es'.          
+        iDestruct "HnS_n" as (es' In Jn Rn) "(HnS_frac & HnS_si & HnS_FP 
+                                & HnS_cl & HnS_oc & HnS_H & HnS_star & Hφ)".
+        iPoseProof (frac_eq with "[$HnP_frac] [$HnS_frac]") as "%".
+        destruct H1 as [Hes [Hc Hb]]. subst es'. subst Cn'. subst Bn'.
         iAssert (inFP γ_f n1)%I as "#HFP_n1".
         { iApply "HnS_cl". iPureIntro. 
           clear -k_in_es. set_solver. }
-        iAssert (⌜(k, Bn !!! k) ∈ outset_KT In n⌝)%I as %outflow_n_n1.
-        { admit. }
+        iAssert (⌜(k, Bn !!! k) ∈ outset_KT In n1⌝)%I as %outflow_n_n1.
+        { iDestruct "HnS_oc" as "(H' & _)".
+          iDestruct "H'" as %H'. iPureIntro. 
+          apply (H' n1 k (Bn !!! k)).
+          repeat split; try done. apply bool_decide_eq_true in Ht.
+          inversion Ht as [H'']. rewrite Cn_val. admit. }
         iAssert (⌜n1 ∈ domm I⌝)%I as %n_in_I.
         { admit. }
         rewrite (big_sepS_delete _ (domm I ∖ {[n]}) n1); last admit.
@@ -444,7 +712,7 @@ Section multicopy.
         iFrame "Hstar'". iExists bn, Cn, Bn.
         iFrame "Hl_n Hlif_n". iExists es, In, Jn, Rn.
         iFrame "∗%". by iApply "HnS_star'". iModIntro.
-        awp_apply (unlockNode_spec_high with "[] [] [HnP_n' node_n]") without "HΦ"; 
+        awp_apply (unlockNode_spec_high with "[] [] [HnP_n' node_n]") without "HΦ";
                         try done. iExists es, T. iFrame.
         iAaccIntro with ""; try eauto with iFrame.
         iIntros "_". iModIntro. iIntros "HΦ". by wp_pures.
@@ -504,6 +772,7 @@ Section multicopy.
   Admitted.        
 *)     
 
+
   Lemma upsert_spec γ_te γ_he γ_s γ_t γ_I γ_J γ_R 
                                   γ_f γ_e γ_c γ_b γ_cir r (k: K) :
     ⊢ ⌜k ∈ KS⌝ -∗ 
@@ -524,7 +793,7 @@ Section multicopy.
     awp_apply lockNode_spec_high; try done.
     iAaccIntro with ""; try eauto with iFrame. 
     iIntros (Cr Br)"HnP_n". iModIntro. wp_pures.
-    iDestruct "HnP_n" as (es T)"(node_n & HnP_frac & HnP_Cn & HnP_t)".
+    iDestruct "HnP_n" as (es T)"(node_n & HnP_frac & HnP_C & HnP_t)".
     iEval (rewrite <-beq_nat_refl) in "HnP_t".
     wp_apply (readClock_spec with "[HnP_t]"); try done.
     iIntros "HnP_t". wp_pures.
@@ -540,18 +809,23 @@ Section multicopy.
     - iDestruct "Hif" as %HCr. wp_pures.
       awp_apply incrementClock_spec. iInv "HInv" as ">H". 
       iDestruct "H" as (T1 H1 I1 J1 R1) "(Hglob & Hstar)".
-      iDestruct "Hglob" as "(MCS & Hs & Ht & HI & HJ & HR & Hf 
+      iDestruct "Hglob" as "(MCS_auth & HH & Ht & HI & HJ & HR & Hf 
                 & Inf_I & Inf_J & Inf_R & _ & Max_ts & domm_IJ & domm_IR)".
-      iAssert (⌜T = T1⌝)%I as %HT. { admit. } replace T1.          
+      iAssert (⌜T = T1⌝)%I as %HT. 
+      { iPoseProof ((own_valid_2 _ _ _) with "[$HnP_t] [$Ht]") as "H'".
+        iDestruct "H'" as %H'. 
+        pose proof (auth_auth_frac_op_inv _ _ _ _ H') as H''.
+        inversion H''. by iPureIntro. } replace T1.          
       iAssert (own γ_t (● (MaxNat T)))%I with "[Ht HnP_t]" as "H".
-      { admit. }          
+      { iCombine "Ht HnP_t" as "H'". done. }          
       iAaccIntro with "H".
       { iIntros "H". iDestruct "H" as "(Ht & HnP_t)".
-        iModIntro. iSplitR "AU HnP_frac HnP_Cn node_n HnP_t".
+        iModIntro. iSplitR "AU HnP_frac HnP_C node_n HnP_t".
         iNext. iExists T, H1, I1, J1, R1. iFrame "∗ #". iFrame. }
       iIntros "H". iDestruct "H" as "(Ht & HnP_t)".
-      iAssert (own γ_s (● (H1 ∪ {[(k,T)]})))%I with "[Hs]" as "Hs".
-      { admit. }
+      iMod (own_update γ_s (● H1) (● (H1 ∪ {[(k,T)]})) with "[$HH]") as "HH".
+      { apply (auth_update_auth _ _ (H1 ∪ {[(k,T)]})).
+        apply gset_local_update. set_solver. } 
       iAssert (maxTS (T+1) (H1 ∪ {[(k, T)]}))%I with "[Max_ts]" as "Max_ts".
       { iDestruct "Max_ts" as %Max_ts. iPureIntro. intros k' t' H.
         assert (((k',t') ∈ H1) ∨ (k' = k ∧ t' = T)) as Hor by set_solver.
@@ -560,26 +834,431 @@ Section multicopy.
           destruct Hor as [_ Hor]. replace t'. lia. }       
       iAssert (⌜set_of_map Cr ⊆ set_of_map Cr'⌝)%I as %Cr_sub_Cr'.
       { admit. }
-      iAssert (own γ_s (◯ set_of_map Cr'))%I with "[HnP_Cn]" as "HnP_Cn".
+      iAssert (own γ_s (◯ set_of_map Cr'))%I with "[HnP_C]" as "HnP_C".
       { admit. }
       iAssert (⌜r ∈ domm I1⌝)%I as %r_in_I.
-      { admit. }
+      { by iPoseProof (inFP_domm _ _ _ with "[$FP_r] [$Hf]") as "H'". }
       rewrite (big_sepS_delete _ (domm I1) r); last by eauto.
       iDestruct "Hstar" as "(H_r & Hstar')".
       iDestruct "H_r" as (br Cr'' Br'')"(Hl_r & Hlif_r & HnS_r)".
-      iAssert (⌜br = true⌝)%I as %Hbr. { admit. } replace br.
+      iAssert (⌜br = true⌝)%I as %Hbr.
+      { destruct br; try done.
+        iDestruct "Hlif_r" as (es' T')"(node' & _)".
+        iPoseProof ((node_sep_star r r) with "[$]") as "%".
+        contradiction. } replace br.
       iDestruct "HnS_r" as (es' Ir Jr Rr) 
             "(HnS_frac & HnS_si & HnS_FP & HnS_cl & HnS_oc & 
-                                        HnS_H & HnS_star & Hφ)".
-      iAssert (⌜es' = es⌝)%I as "%".  
-      { admit. } subst es'.      
-      iAssert (⌜Cr'' = Cr⌝)%I as "%".  
-      { admit. } subst Cr''.      
-      iAssert (⌜Br'' = Br⌝)%I as "%".  
-      { admit. } subst Br''.
-      case_eq (Cr !! k).
-      + intros t Cr_k.
+                                        HnS_if & HnS_star & Hφ)".
+      iPoseProof (frac_eq with "[$HnP_frac] [$HnS_frac]") as "%".
+      destruct H as [Hes [Hc Hb]]. subst es'. subst Cr''. subst Br''.
+      destruct (decide (Cr !!! k = 0)) as [ Cr_k | Cr_k ]; last first.
+      + set (Br' := <[k := T]>Br).
+        assert (Br' = <[k := T]>Br) as HBr'. try done.
+        iAssert (⌜Br' = map_of_set (H1 ∪ {[(k, T)]})⌝)%I as %Br'_eq_H1.
+        { admit. }
+        assert (∀ k', k' ≠ k → Br' !!! k' = Br !!! k') as HBr_neq.
+        { intros k' Hk'. rewrite /(Br !!! k').
+          rewrite /(Br' !!! k'). 
+          unfold finmap_lookup_total.
+          unfold inhabitant. simpl.
+          assert (Br' !! k' = Br !! k') as HBr.
+          { by apply lookup_insert_ne. } 
+          by rewrite HBr. }
+        assert (Br' !!! k = T) as HBr'_k.
+        { apply lookup_total_insert. }          
+        iAssert ([∗ set] k0 ∈ KS, own (γ_cir r k0) 
+                    (● {| max_nat_car := Br' !!! k0 |}))%I 
+            with "[HnS_star]" as "HnS_star".
+        { admit. }
+        iMod ((frac_update γ_e γ_c γ_b r es Cr Br es Cr' Br') 
+                    with "[$HnP_frac $HnS_frac]") as "(HnP_frac & HnS_frac)".
+        assert ((∃ n, k ∈ es !!! n ∧ n ≠ r) ∨ (∀ n, k ∉ es !!! n)) as Hes.
+        { admit. } destruct Hes as [Hes | Hes].
+        * destruct Hes as [n [k_in_es n_neq_r]].
+          set (Jr'_temp := outflow_delete_KT Jr n k (Cr !!! k)).
+          set (Jr' := outflow_insert_KT Jr'_temp n k T).
+          iAssert (outflow_constraints r Ir Jr' Rr es Cr' Br')%I 
+                    with "[HnS_oc]" as "HnS_oc".
+          { iDestruct "HnS_oc" as "(% & % & %)".
+            rename H into OC_1. rename H2 into OC_2.
+            rename H3 into OC_3. 
+            iPureIntro. split; last split; try done.
+            - intros n' k' t'. split.
+              + intros Hout.
+                apply OC_1 in Hout.
+                destruct Hout as [Hout1 [Hout2 Hout3]].
+                destruct (decide (k' = k)).
+                * replace k' in Hout2.
+                  contradiction.
+                * repeat split; try done.
+                  rewrite /(Cr' !!! k'). 
+                  unfold finmap_lookup_total.
+                  replace Cr'. rewrite lookup_insert_ne; try done.
+                  rewrite /(Br' !!! k'). 
+                  unfold finmap_lookup_total.
+                  rewrite HBr'. rewrite lookup_insert_ne; try done.
+              + intros [Hout1 [Hout2 Hout3]].
+                apply OC_1. split; try done.
+                destruct (decide (k' = k)).
+                * replace k'.
+                  rewrite e in Hout2. replace Cr' in Hout2.
+                  rewrite lookup_total_insert in Hout2.
+                  admit. (* Contradiction: T = 0 *)
+                * rewrite /(Cr' !!! k') in Hout2.
+                  unfold finmap_lookup_total in Hout2.
+                  replace Cr' in Hout2. 
+                  rewrite lookup_insert_ne in Hout2; try done.
+                  rewrite /(Br' !!! k') in Hout3.
+                  unfold finmap_lookup_total in Hout3; try done.
+                  rewrite HBr' in Hout3. 
+                  rewrite lookup_insert_ne in Hout3; try done.
+            - intros n' k' t'.
+              destruct (decide (n' = n)).
+              + assert (outset_KT Jr' n = 
+                      (outset_KT Jr n ∖ {[k, Cr !!! k]}) ∪ {[k, T]}) as Outset.
+                { pose proof outflow_insert_outset_KT Jr'_temp n k T Jr' as Houts.
+                  assert (Jr' = outflow_insert_KT Jr'_temp n k T) as HJr' by done.
+                  pose proof Houts HJr' n' as [Hp _].
+                  pose proof Hp e as Hp.
+                  pose proof outflow_delete_outset_KT Jr n k (Cr !!! k) Jr'_temp 
+                    as Houts'. 
+                  assert (Jr'_temp = outflow_delete_KT Jr n k (Cr !!! k)) 
+                    as HJr_t by done.  
+                  pose proof Houts' HJr_t n' as [Hp' _].
+                  pose proof Hp' e as Hp'.
+                  rewrite e in Hp.
+                  rewrite e in Hp'.
+                  by rewrite Hp' in Hp. }
+                replace n'.  
+                assert ((k',t') ∈ outset_KT Jr' n → 
+                       ((k',t') ∈ outset_KT Jr n) ∨ (k',t') = (k, T)) as Hkt'.
+                { intros Hout. rewrite Outset in Hout.
+                  set_solver. }
+                split.
+                * intros Hout. pose proof Hkt' Hout as Hkt'.
+                  destruct Hkt' as [Hkt' | Hkt'].
+                  ** apply OC_2 in Hkt'.
+                     destruct Hkt' as [Hkt'_1 Hkt'_2]. 
+                     split; try done.
+                     destruct (decide (k' = k)).
+                     rewrite e0 in Hkt'_2.
+                     rewrite e0 in Hout.
+                     rewrite <-Hkt'_2 in Hout.
+                     assert ((k, Cr !!! k) ∉ outset_KT Jr' n).
+                     { clear -Outset.
+                       assert (Cr !!! k ≠ T). admit.
+                       set_solver. }
+                     contradiction.
+                     replace Cr'. 
+                     rewrite lookup_total_insert_ne; try done.
+                  ** inversion Hkt'.
+                     repeat split; try done.
+                     replace Cr'.
+                     rewrite lookup_total_insert; try done.
+                * intros [Hk1 Hk2].
+                  destruct (decide (k' = k)).
+                  ** replace k'.
+                     rewrite e0 in Hk1.
+                     rewrite e0 in Hk2.
+                     replace Cr' in Hk2. 
+                     rewrite lookup_total_insert in Hk2.
+                     replace t'. rewrite Outset.
+                     set_solver.
+                  ** replace Cr' in Hk2.
+                     rewrite lookup_total_insert_ne in Hk2; try done.
+                     assert (k' ∈ es !!! n ∧ Cr !!! k' = t') as Hkt; try done.
+                     apply OC_2 in Hkt.
+                     rewrite Outset.
+                     clear -Hkt n0. set_solver.
+              + assert (outset_KT Jr' n' = outset_KT Jr n') as Outset.
+                { pose proof outflow_insert_outset_KT Jr'_temp n k T Jr' as Houts.
+                  assert (Jr' = outflow_insert_KT Jr'_temp n k T) as HJr' by done.
+                  pose proof Houts HJr' n' as [_ Hp].
+                  pose proof Hp n0 as Hp.
+                  pose proof outflow_delete_outset_KT Jr n k (Cr !!! k) Jr'_temp 
+                    as Houts'. 
+                  assert (Jr'_temp = outflow_delete_KT Jr n k (Cr !!! k)) 
+                    as HJr_t by done.  
+                  pose proof Houts' HJr_t n' as [_ Hp'].
+                  pose proof Hp' n0 as Hp'.
+                  by rewrite Hp' in Hp. }
+                rewrite Outset.
+                split.
+                * intros Hout.
+                  apply OC_2 in Hout.
+                  destruct Hout as [Hout1 Hout2].
+                  split; try done.
+                  destruct (decide (k' = k)).
+                  ** rewrite e in Hout1.
+                     admit.
+                  ** replace Cr'.
+                     rewrite lookup_total_insert_ne; try done.
+                * intros [Hout1 Hout2].
+                  destruct (decide (k' = k)).
+                  ** rewrite e in Hout1.
+                     admit.
+                  ** replace Cr' in Hout2.
+                     rewrite lookup_total_insert_ne in Hout2; try done.
+                     apply OC_2.
+                     split; try done. }
+          iAssert (inFP γ_f n)%I as "#FP_n".
+          { iApply "HnS_cl". iPureIntro.
+            clear -k_in_es. set_solver. }
+          iAssert (⌜n ∈ domm I1⌝)%I as %n_in_I.
+          { by iPoseProof (inFP_domm _ _ _ with "[$FP_n] [$Hf]") as "H'". }
+          rewrite (big_sepS_delete _ (domm I1 ∖ {[r]}) n); last by set_solver.
+          iDestruct "Hstar'" as "(H_n & Hstar')".
+          iDestruct "H_n" as (bn Cn Bn)"(Hl_n & Hlif_n & HnS_n)".
+          iDestruct "HnS_n" as (es_n In Jn Rn) 
+            "(HnS_fracn & HnS_sin & HnS_FPn & HnS_cln & HnS_ocn & 
+                                        HnS_ifn & HnS_starn & Hφn)".
+          set (Jn'_temp := inflow_delete_KT Jn n k (Cr !!! k)).
+          set (Jn' := inflow_insert_KT Jn'_temp n k T).
+          iAssert (outflow_constraints n In Jn' Rn es_n Cn Bn)%I
+            with "[HnS_ocn]" as "HnS_ocn".
+          { iDestruct "HnS_ocn" as "(% & % & %)".
+            rename H into OC_1. rename H2 into OC_2.
+            rename H3 into OC_3. 
+            iPureIntro. split; last split; try done. }
+          iAssert (singleton_interfaces_ghost_state γ_I γ_J γ_R r Ir Jr' Rr
+            ∗ singleton_interfaces_ghost_state γ_I γ_J γ_R n In Jn' Rn)%I 
+                    with "[HnS_si HnS_sin]" as "(HnS_si & HnS_sin)".
+          { unfold singleton_interfaces_ghost_state. 
+            iDestruct "HnS_si" as "(HrI & HrJ & HrR & Domm_rI & Domm_rJ & Domm_rR)".
+            iDestruct "HnS_sin" as "(HnI & HnJ & HnR & Domm_nI & Domm_nJ & Domm_nR)".
+            assert (domm Jn' = domm Jn).
+            { assert (Jn'_temp = inflow_delete_KT Jn n k (Cr !!! k)) 
+                          as HJn't by done.
+              assert (Jn' = inflow_insert_KT Jn'_temp n k T) as HJn' by done.
+              assert (domm Jn' = domm Jn'_temp) as H'.
+              apply (inflow_insert_domm _ n k T); try done.
+              assert (domm Jn'_temp = domm Jn) as H''.
+              apply (inflow_delete_domm _ n k (Cr !!! k)); try done.
+              by rewrite H'. } 
+            rewrite H. iFrame.
+            iCombine "HrJ HnJ" as "HrnJ".
+            assert (Jr ⋅ Jn = Jr' ⋅ Jn') as H'.
+            { assert (Jr ⋅ Jn = Jr'_temp ⋅ Jn'_temp) as H'.
+              { apply (flow_delete_eq_KT Jr Jr'_temp _ _ n k (Cr !!! k));
+                         try done. }
+              assert (Jr'_temp ⋅ Jn'_temp = Jr' ⋅ Jn') as H''.
+              { apply (flow_insert_eq_KT Jr'_temp Jr' _ _ n k T);
+                         try done. }
+              by rewrite H'. }            
+            iEval (rewrite H') in "HrnJ".
+            iEval (rewrite auth_frag_op) in "HrnJ".
+            iDestruct "HrnJ" as "(HrJ & HnJ)". iFrame. }
+          iEval (rewrite <-beq_nat_refl) in "HnS_if".
+          iDestruct "HnS_if" as "(H' & H'' & H''')".
+          iDestruct "H'" as %Br_eq_H1. 
+          iDestruct "H''" as %Infz_rI.
+          iDestruct "H'''" as %Infz_rJ.
+          iDestruct "Inf_R" as %Inf_R.
+          iPoseProof ((auth_own_incl γ_R R1 Rr) with "[HR HnS_si]")
+              as (Ro) "%". 
+          { unfold singleton_interfaces_ghost_state.
+            iDestruct "HnS_si" as "(_ & _ & H' & _)". 
+            iFrame. } rename H into Incl_R1.
+          iPoseProof (own_valid with "HR") as "%".
+          rename H into Valid_R1.
+          iAssert (⌜domm Rr = {[r]}⌝)%I as "%".
+          { by iDestruct "HnS_si" as "(_&_&_&_&_&H')". }
+          rename H into Domm_Rr.
+          iAssert (φ1 Br' Cr' Ir ∗ φ2 r Br' Ir ∗ φ3 r Br' Jr' ∗ φ4 r Br' Rr 
+                  ∗ φ5 r Rr)%I with "[Hφ]" as "Hφ".
+          { iDestruct "Hφ" as %Hφ. 
+            destruct Hφ as [Hφ1 [Hφ2 [Hφ3 [Hφ4 Hφ5]]]].
+            iPureIntro. repeat split; try done.
+            - intros k'. pose proof Hφ1 k' as Hφ1.
+              destruct Hφ1 as [Hφ1 | Hφ1].
+              by left.
+              destruct (decide (k' = k)).
+              replace k'. right.
+              replace Cr'. rewrite HBr'.
+              rewrite lookup_total_insert.
+              by rewrite lookup_total_insert.
+              right.    
+              replace Cr'. rewrite HBr'.
+              rewrite lookup_total_insert_ne; try done.
+              rewrite lookup_total_insert_ne; try done.
+            - intros k' t' Hins.
+              pose proof Infz_rI r as Infz_rI.
+              rewrite Infz_rI in Hins.
+              exfalso. clear -Hins. set_solver.
+            - intros k' t' Hins.
+              pose proof Infz_rJ r as Infz_rJ.
+              assert (inset_KT Jr' r = inset_KT Jr r) as H'.
+              { assert (inset_KT Jr'_temp r = inset_KT Jr r) as H'.
+                apply (outflow_delete_inf_eq_KT _ n k (Cr !!! k)); try done.
+                assert (inset_KT Jr' r = inset_KT Jr'_temp r) as H''.
+                apply (outflow_insert_inf_eq_KT _ n k T); try done.
+                by rewrite <-H'. }
+              rewrite H' in Hins. rewrite Infz_rJ in Hins.
+              exfalso. clear -Hins. set_solver.
+            - intros k'. right.
+              apply (inset_monotone R1 Rr Ro); try done.
+              by rewrite <-auth_auth_valid.
+              pose proof Inf_R r k' as Inf_R.
+              by rewrite <-beq_nat_refl in Inf_R.
+              rewrite Domm_Rr. clear. set_solver. } 
+          iAssert (φ1 Bn Cn In ∗ φ2 n Bn In ∗ φ3 n Bn Jn' ∗ φ4 n Bn Rn 
+                  ∗ φ5 n Rn)%I with "[Hφn]" as "Hφn".
+          { iDestruct "Hφn" as %Hφ. 
+            destruct Hφ as [Hφ1 [Hφ2 [Hφ3 [Hφ4 Hφ5]]]].
+            iPureIntro. repeat split; try done.
+            intros k' t'. 
+            assert (inset_KT Jn' n = 
+                      (inset_KT Jn n ∖ {[k, Cr !!! k]}) ∪ {[k, T]}) as Inset.
+            { pose proof inflow_insert_outset_KT Jn'_temp n k T Jn' as Hin.
+              assert (Jn' = inflow_insert_KT Jn'_temp n k T) as HJn' by done.
+              pose proof Hin HJn' n as [Hp _].
+              assert (n = n) as H' by done.
+              pose proof Hp H' as Hp.
+              pose proof inflow_delete_outset_KT Jn n k (Cr !!! k) Jn'_temp as Hin'. 
+              assert (Jn'_temp = inflow_delete_KT Jn n k (Cr !!! k)) 
+                    as HJn_t by done.  
+              pose proof Hin' HJn_t n as [Hp' _].
+              pose proof Hp' H' as Hp'.
+              by rewrite Hp' in Hp. }
+              assert ((k',t') ∈ inset_KT Jn' n → 
+                       ((k',t') ∈ inset_KT Jn n) ∨ (k',t') = (k, T)) as Hkt'.
+              { intros Hin. rewrite Inset in Hin. set_solver. }
+              intros Hin. apply Hkt' in Hin.
+              destruct Hin as [Hin | Hin].
+              by pose proof Hφ3 k' t' Hin as Hφ3.
+              inversion Hin.
+              admit.
+          }  
+          iMod "AU" as (t' H')"[MCS [_ Hclose]]".
+          iAssert (⌜t' = T⌝)%I as %Ht'. 
+          { iPoseProof ((auth_agree γ_te) with "[MCS_auth] [MCS]") as "%".
+            unfold MCS_auth. by iDestruct "MCS_auth" as "(H' & _)".
+            by iDestruct "MCS" as "(H' & _)".
+            by iPureIntro. } replace t'.
+          iAssert (⌜H' = H1⌝)%I as %H1'.
+          { iPoseProof ((auth_agree' γ_he) with "[MCS_auth] [MCS]") as "%".
+            unfold MCS_auth. by iDestruct "MCS_auth" as "(_ & H'')".
+            by iDestruct "MCS" as "(_ & H')".
+            by iPureIntro. } replace H'.
+          iDestruct "MCS" as "(MCS◯t & MCS◯h)".
+          iDestruct "MCS_auth" as "(MCS●t & MCS●h)".
+          iMod ((auth_update γ_te (T+1) T T) with "MCS●t MCS◯t") 
+                                              as "(MCS●t & MCS◯t)".
+          iMod ((auth_update' γ_he (H1 ∪ {[(k, T)]}) H1 H1) with "MCS●h MCS◯h") 
+                                              as "(MCS●h & MCS◯h)".
+          iCombine "MCS◯t MCS◯h" as "MCS".
+          iCombine "MCS●t MCS●h" as "MCS_auth".
+          iMod ("Hclose" with "MCS") as "HΦ".            
+          
+          
+          iModIntro.
+          iSplitR "HΦ node_n HnP_t HnP_C HnP_frac".
+          { iNext. iExists (T+1), (H1 ∪ {[(k, T)]}), I1, J1, R1.
+            iFrame "∗ %".   
+            rewrite (big_sepS_delete _ (domm I1) r); last by eauto.
+            iSplitL "Hl_r Hlif_r HnS_cl HnS_star Hφ HnS_frac HnS_oc HnS_si".
+            { iExists true, Cr', Br'. iFrame.
+              unfold nodeShared. iExists es, Ir, Jr', Rr.
+              iFrame "∗#". iEval (rewrite <-beq_nat_refl). 
+              iFrame "%∗". }        
+            rewrite (big_sepS_delete _ (domm I1 ∖ {[r]}) n); last by set_solver.
+            iSplitL "Hl_n Hlif_n HnS_cln HnS_starn Hφn HnS_fracn HnS_ocn 
+                        HnS_sin HnS_ifn".
+            { iExists bn, Cn, Bn. iFrame. iExists es_n, In, Jn', Rn.
+              iFrame "∗#". assert (n =? r = false) as Hnr. 
+              { by rewrite beq_nat_false_iff. } 
+              by rewrite Hnr. }
+            iApply (big_opS_proper (λ y, ∃ (bn0 : bool) (Cn0 Bn0 : gmap K natUR),
+                                      lockLoc y ↦ #bn0
+                                    ∗ (if bn0 then True else
+                                       nodePred γ_e γ_c γ_b γ_t γ_s r y Cn0 Bn0)
+                                    ∗ nodeShared γ_I γ_J γ_R γ_e γ_c γ_b γ_f γ_cir
+                                              r y Cn0 Bn0 H1 )%I
+                                   (λ y, ∃ (bn0 : bool) (Cn0 Bn0 : gmap K natUR),
+                                      lockLoc y ↦ #bn0
+                                    ∗ (if bn0 then True else
+                                       nodePred γ_e γ_c γ_b γ_t γ_s r y Cn0 Bn0)
+                                    ∗ nodeShared γ_I γ_J γ_R γ_e γ_c γ_b γ_f γ_cir
+                                              r y Cn0 Bn0 (H1 ∪ {[(k, T)]}) )%I
+                                   (domm I1 ∖ {[r]} ∖ {[n]})); try done.
+            intros y y_dom. assert (y ≠ r) as Hy by set_solver. iFrame. iSplit;
+            iIntros "Hstar"; iDestruct "Hstar" as (b C B)"(Hl & Hlif & HnS)";
+            iExists b, C, B; iFrame; 
+            iDestruct "HnS" as (esy Iy Jy Ry)"(HnS_frac & HnS_si & HnS_FP 
+                          & HnS_cl & HnS_oc & HnS_if & HnS_star & Hφ)";
+            iExists esy, Iy, Jy, Ry; iFrame; 
+            assert (y =? r = false) as Hyr by (rewrite beq_nat_false_iff; done);
+            iEval (rewrite Hyr); done. } 
+          wp_pures.  
+          awp_apply (unlockNode_spec_high with "[] [] [HnP_t HnP_C HnP_frac node_n]")
+                without "HΦ"; try done. iExists es, (T + 1). iFrame.
+                by iEval (rewrite <-beq_nat_refl).
+          iAaccIntro with ""; try eauto with iFrame.
+          
+          
+          
+        * iAssert (outflow_constraints r Ir Jr Rr es Cr' Br')%I 
+                    with "[HnS_oc]" as "HnS_oc".
+          { admit. }
+          iAssert (φ1 Br' Cr' Ir ∗ φ2 r Br' Ir ∗ φ3 r Br' Jr ∗ φ4 r Br' Rr 
+                  ∗ φ5 r Rr)%I with "[Hφ]" as "Hφ".
+          { admit. }  
+          iMod "AU" as (t' H')"[MCS [_ Hclose]]".
+          iAssert (⌜t' = T⌝)%I as %Ht'. { admit. } replace t'.
+          iAssert (⌜H' = H1⌝)%I as %H1'. { admit. } replace H'.
+          iAssert (MCS γ_te γ_he (T+1) (H1 ∪ {[(k, T)]}) ∗
+                   MCS_auth γ_te γ_he (T+1) (H1 ∪ {[(k, T)]}))%I
+            with "[MCS MCS_auth]" as "(MCS & MCS_auth)".
+          { admit. }
+          iMod ("Hclose" with "MCS") as "HΦ".            
+                    
+          
+          
+          iModIntro.
+          iSplitR "HΦ node_n HnP_t HnP_C HnP_frac".
+          { iNext. iExists (T+1), (H1 ∪ {[(k, T)]}), I1, J1, R1.
+            iFrame.   
+            rewrite (big_sepS_delete _ (domm I1) r); last by eauto.
+            iSplitL "Hl_r Hlif_r HnS_cl HnS_star Hφ HnS_frac HnS_oc HnS_si HnS_if".
+            { iExists true, Cr', Br'. iFrame.
+              unfold nodeShared. iExists es, Ir, Jr, Rr.
+              iFrame "∗#". iEval (rewrite <-beq_nat_refl) in "HnS_if".
+              iDestruct "HnS_if" as "(_ & HnS_if)".
+              iEval (rewrite <-beq_nat_refl). iFrame "%∗". }        
+            iApply (big_opS_proper (λ y, ∃ (bn0 : bool) (Cn0 Bn0 : gmap K natUR),
+                                      lockLoc y ↦ #bn0
+                                    ∗ (if bn0 then True else
+                                       nodePred γ_e γ_c γ_b γ_t γ_s r y Cn0 Bn0)
+                                    ∗ nodeShared γ_I γ_J γ_R γ_e γ_c γ_b γ_f γ_cir
+                                              r y Cn0 Bn0 H1 )%I
+                                   (λ y, ∃ (bn0 : bool) (Cn0 Bn0 : gmap K natUR),
+                                      lockLoc y ↦ #bn0
+                                    ∗ (if bn0 then True else
+                                       nodePred γ_e γ_c γ_b γ_t γ_s r y Cn0 Bn0)
+                                    ∗ nodeShared γ_I γ_J γ_R γ_e γ_c γ_b γ_f γ_cir
+                                              r y Cn0 Bn0 (H1 ∪ {[(k, T)]}) )%I
+                                   (domm I1 ∖ {[r]})); try done.
+            intros y y_dom. assert (y ≠ r) as Hy by set_solver. iFrame. iSplit;
+            iIntros "Hstar"; iDestruct "Hstar" as (b C B)"(Hl & Hlif & HnS)";
+            iExists b, C, B; iFrame; 
+            iDestruct "HnS" as (esy Iy Jy Ry)"(HnS_frac & HnS_si & HnS_FP 
+                          & HnS_cl & HnS_oc & HnS_if & HnS_star & Hφ)";
+            iExists esy, Iy, Jy, Ry; iFrame; 
+            assert (y =? r = false) as Hyr by (rewrite beq_nat_false_iff; done);
+            iEval (rewrite Hyr); done. } 
+          wp_pures.  
+          awp_apply (unlockNode_spec_high with "[] [] [HnP_t HnP_C HnP_frac node_n]")
+                without "HΦ"; try done. iExists es, (T + 1). iFrame.
+                by iEval (rewrite <-beq_nat_refl).
+          iAaccIntro with ""; try eauto with iFrame.
+      + intros Cr_k.
         set (Br' := <[k := T]>Br).
+        iAssert (⌜Br' = map_of_set (H1 ∪ {[(k, T)]})⌝)%I as %Br_eq_H1.
+        { admit. }
+        iAssert ([∗ set] k0 ∈ KS, own (γ_cir r k0) 
+                    (● {| max_nat_car := Br' !!! k0 |}))%I 
+            with "[HnS_star]" as "HnS_star".
+        { admit. }     
         iAssert (frac_ghost_state γ_e γ_c γ_b r es Cr' Br' ∗ 
                     frac_ghost_state γ_e γ_c γ_b r es Cr' Br')%I 
               with "[HnP_frac HnS_frac]" as "(HnP_frac & HnS_frac)".
@@ -588,20 +1267,100 @@ Section multicopy.
         { admit. } destruct Hes as [Hes | Hes].
         * destruct Hes as [n [k_in_es n_neq_r]].
           set (Jr'_out_r := (nzmap_imerge 
-             (λ k' a1 _, if (decide (k' = (k, t))) then 0 else 
-                         if (decide (k' = (k, T))) then 1 else a1) (out Jr n) (∅)): (KT_multiset)).
+             (λ k' a1 _, if (decide (k' = (k, T))) then 1 else a1)
+                         (out Jr n) (∅)): (KT_multiset)).
           set (Jr'_out := (nzmap_imerge 
                       (λ k' a1 _, if (decide (k = r)) then Jr'_out_r else a1)
                       (out_map Jr) (∅)) : (nzmap Node KT_multiset)).
-          set (Jr' := ({| infR := 
-          (inf_map Jr: gmap Node KT_multiset) ; 
-           outR := (Jr'_out: nzmap Node KT_multiset) |})).
-(*
-          set (Jr1 : (KT_flowint_ur K) := Jr' : (KT_flowint_ur)).  
-          iAssert (outflow_constraints r Ir Jr' Rr es Cr' Br')%I 
+          set (Jr1' := ({| infR := inf_map Jr ; outR := Jr'_out |})).
+          set (Jr' := ∅: (KT_flowint_ur K)).
+          set (Ir' := ∅: (KT_flowint_ur K)).
+          iAssert (outflow_constraints r Ir' Jr' Rr es Cr' Br')%I 
                     with "[HnS_oc]" as "HnS_oc".
           { admit. }
-*)
+          iAssert (inFP γ_f n)%I as "#FP_n". 
+          { iApply "HnS_cl". iPureIntro.
+            clear -k_in_es. set_solver. }
+          iAssert (⌜n ∈ domm I1⌝)%I as %n_in_I.
+          { admit. }
+          rewrite (big_sepS_delete _ (domm I1 ∖ {[r]}) n); last by set_solver.
+          iDestruct "Hstar'" as "(H_n & Hstar')".
+          iDestruct "H_n" as (bn Cn Bn)"(Hl_n & Hlif_n & HnS_n)".
+          iDestruct "HnS_n" as (es_n In Jn Rn) 
+            "(HnS_fracn & HnS_sin & HnS_FPn & HnS_cln & HnS_ocn & 
+                                        HnS_ifn & HnS_starn & Hφn)".
+          set (Jn' := ∅: (KT_flowint_ur K)).
+          set (In' := ∅: (KT_flowint_ur K)).
+          iAssert (singleton_interfaces_ghost_state γ_I γ_J γ_R r Ir' Jr' Rr
+            ∗ singleton_interfaces_ghost_state γ_I γ_J γ_R n In' Jn' Rn)%I 
+                    with "[HnS_si HnS_sin]" as "(HnS_si & HnS_sin)".
+          { admit. }          
+          iAssert (outflow_constraints n In' Jn' Rn es_n Cn Bn)%I
+            with "[HnS_ocn]" as "HnS_ocn".
+          { admit. }
+          iAssert (φ1 Br' Cr' Ir' ∗ φ2 r Br' Ir' ∗ φ3 r Br' Jr' ∗ φ4 r Br' Rr 
+                  ∗ φ5 r Rr)%I with "[Hφ]" as "Hφ".
+          { admit. }  
+          iAssert (φ1 Bn Cn In' ∗ φ2 n Bn In' ∗ φ3 n Bn Jn' ∗ φ4 n Bn Rn 
+                  ∗ φ5 n Rn)%I with "[Hφn]" as "Hφn".
+          { admit. }  
+          iMod "AU" as (t' H')"[MCS [_ Hclose]]".
+          iAssert (⌜t' = T⌝)%I as %Ht'. { admit. } replace t'.
+          iAssert (⌜H' = H1⌝)%I as %H1'. { admit. } replace H'.
+          iAssert (MCS γ_te γ_he (T+1) (H1 ∪ {[(k, T)]}) ∗
+                   MCS_auth γ_te γ_he (T+1) (H1 ∪ {[(k, T)]}))%I
+            with "[MCS MCS_auth]" as "(MCS & MCS_auth)".
+          { admit. }
+          iMod ("Hclose" with "MCS") as "HΦ".            
+                    
+          
+          
+          iModIntro.
+          iSplitR "HΦ node_n HnP_t HnP_C HnP_frac".
+          { iNext. iExists (T+1), (H1 ∪ {[(k, T)]}), I1, J1, R1.
+            iFrame.   
+            rewrite (big_sepS_delete _ (domm I1) r); last by eauto.
+            iSplitL "Hl_r Hlif_r HnS_cl HnS_star Hφ HnS_frac HnS_oc HnS_si HnS_if".
+            { iExists true, Cr', Br'. iFrame.
+              unfold nodeShared. iExists es, Ir', Jr', Rr.
+              iFrame "∗#". iEval (rewrite <-beq_nat_refl) in "HnS_if".
+              iDestruct "HnS_if" as "(_ & HnS_if)".
+              iEval (rewrite <-beq_nat_refl). iFrame "%∗".
+              unfold inflow_zero. admit. }        
+            rewrite (big_sepS_delete _ (domm I1 ∖ {[r]}) n); last by set_solver.
+            iSplitL "Hl_n Hlif_n HnS_cln HnS_starn Hφn HnS_fracn HnS_ocn 
+                        HnS_sin HnS_ifn".
+            { iExists bn, Cn, Bn. iFrame. iExists es_n, In', Jn', Rn.
+              iFrame "∗#". assert (n =? r = false) as Hnr. 
+              { by rewrite beq_nat_false_iff. } 
+              by rewrite Hnr. }
+            iApply (big_opS_proper (λ y, ∃ (bn0 : bool) (Cn0 Bn0 : gmap K natUR),
+                                      lockLoc y ↦ #bn0
+                                    ∗ (if bn0 then True else
+                                       nodePred γ_e γ_c γ_b γ_t γ_s r y Cn0 Bn0)
+                                    ∗ nodeShared γ_I γ_J γ_R γ_e γ_c γ_b γ_f γ_cir
+                                              r y Cn0 Bn0 H1 )%I
+                                   (λ y, ∃ (bn0 : bool) (Cn0 Bn0 : gmap K natUR),
+                                      lockLoc y ↦ #bn0
+                                    ∗ (if bn0 then True else
+                                       nodePred γ_e γ_c γ_b γ_t γ_s r y Cn0 Bn0)
+                                    ∗ nodeShared γ_I γ_J γ_R γ_e γ_c γ_b γ_f γ_cir
+                                              r y Cn0 Bn0 (H1 ∪ {[(k, T)]}) )%I
+                                   (domm I1 ∖ {[r]} ∖ {[n]})); try done.
+            intros y y_dom. assert (y ≠ r) as Hy by set_solver. iFrame. iSplit;
+            iIntros "Hstar"; iDestruct "Hstar" as (b C B)"(Hl & Hlif & HnS)";
+            iExists b, C, B; iFrame; 
+            iDestruct "HnS" as (esy Iy Jy Ry)"(HnS_frac & HnS_si & HnS_FP 
+                          & HnS_cl & HnS_oc & HnS_if & HnS_star & Hφ)";
+            iExists esy, Iy, Jy, Ry; iFrame; 
+            assert (y =? r = false) as Hyr by (rewrite beq_nat_false_iff; done);
+            iEval (rewrite Hyr); done. } 
+          wp_pures.  
+          awp_apply (unlockNode_spec_high with "[] [] [HnP_t HnP_C HnP_frac node_n]")
+                without "HΦ"; try done. iExists es, (T + 1). iFrame.
+                by iEval (rewrite <-beq_nat_refl).
+          iAaccIntro with ""; try eauto with iFrame.
+                    
   Admitted.
 
 End multicopy.             
